src/lowparse/steel_c_array/LowParse.SteelST.ArrayPtr.fst
@@ -1,0 +1,337 @@
+module LowParse.SteelST.ArrayPtr
+module STC = Steel.ST.C.Types
+
+let t elt = STC.array_ptr (STC.scalar elt)
+
+[@@erasable]
+noeq
+type array elt = {
+  array_ptr: STC.array (STC.scalar elt);
+  array_perm: Steel.FractionalPermission.perm;
+//  array_base_len: (len: SZ.t { SZ.v len == SA.base_len (STC.base (STC.array_ptr_of array_ptr)) });
+}
+
+let len x = SZ.uint_to_t (STC.array_length x.array_ptr)
+
+let array_perm x = x.array_perm
+
+[@@erasable]
+noeq
+type v t = {
+  v_array: array t;
+  v_contents: Seq.lseq t (length v_array);
+}
+
+let array_of x = x.v_array
+let contents_of x = x.v_contents
+
+let array_contents_inj _ _ = ()
+
+let mk_full_scalar_seq_index (#t: Type) (s: Seq.seq t) (i: nat { i < Seq.length s }) : GTot (STC.scalar_t t) =
+  STC.mk_scalar (Seq.index s i)
+
+let mk_full_scalar_seq (#t: Type) (s: Seq.seq t) : GTot (Seq.seq (STC.scalar_t t)) =
+  Seq.init_ghost (Seq.length s) (mk_full_scalar_seq_index s)
+
+let mk_scalar_seq (#t: Type) (p: perm) (s: Seq.seq t) : GTot (Seq.seq (STC.scalar_t t)) =
+  STC.mk_fraction_seq (STC.scalar t) (mk_full_scalar_seq s) p
+
+[@__reduce__]
+let arrayptr1 (#elt: _) (v: v elt) (s: Ghost.erased (Seq.seq (STC.scalar_t elt))) : Tot vprop =
+    STC.array_pts_to v.v_array.array_ptr s
+
+[@__reduce__]
+let arrayptr0 (#elt: _) (r: t elt) (v: v elt) : Tot vprop =
+  exists_ (fun s ->
+    arrayptr1 v s `star` pure (
+    Ghost.reveal s `Seq.equal` mk_scalar_seq v.v_array.array_perm v.v_contents /\
+    STC.array_ptr_of v.v_array.array_ptr == r /\
+    (Seq.length v.v_contents > 0 ==> v.v_array.array_perm `lesser_equal_perm` full_perm)
+  ))
+
+let arrayptr r v = arrayptr0 r v
+    
+let adjacent x1 x2 =
+  x1.array_perm == x2.array_perm /\
+  STC.array_ptr_of x2.array_ptr == STC.array_ref_shift (STC.array_ptr_of x1.array_ptr) (len x1)
+
+let merge x1 x2 = {
+  array_ptr = (| STC.array_ptr_of x1.array_ptr, Ghost.hide (len x1 `SZ.add` len x2) |);
+  array_perm = x1.array_perm;
+//  array_base_len = x1.array_base_len;
+}
+
+let merge_assoc x1 x2 x3 =
+  STC.array_ref_shift_assoc (STC.array_ptr_of x1.array_ptr) (len x1) (len x2)
+
+let join #_ #a #vl #vr al ar =
+  rewrite (arrayptr al vl) (arrayptr0 al vl);
+  rewrite (arrayptr ar vr) (arrayptr0 ar vr);
+  let _ = gen_elim () in
+  let res = {
+    v_array = merge (array_of vl) (array_of vr);
+    v_contents = Seq.append vl.v_contents vr.v_contents;
+  }
+  in
+  STC.array_join res.v_array.array_ptr vl.v_array.array_ptr vr.v_array.array_ptr (len (array_of vl));
+  rewrite (arrayptr0 al res) (arrayptr al res);
+  res
+
+unfold
+let gsplit_post
+  (#a:Type) (value: v a) (x: t a) (i:SZ.t)
+  (res: t a)
+  (vl vr: v a)
+: GTot prop
+=
+            SZ.v i <= length (array_of value) /\
+            merge_into (array_of vl) (array_of vr) (array_of value) /\
+            contents_of' vl `Seq.equal` seq_slice (contents_of' value) 0 (SZ.v i) /\
+            length (array_of vl) == SZ.v i /\
+            length (array_of vr) == length (array_of value) - SZ.v i /\
+            contents_of' vr `Seq.equal` seq_slice (contents_of' value) (SZ.v i) (length (array_of value)) /\
+            contents_of' value `Seq.equal` (contents_of' vl `Seq.append` contents_of' vr) /\
+            (SZ.v i == 0 ==> Ghost.reveal res == x)
+
+let gsplit #_ #_ #v x i =
+  rewrite (arrayptr x v) (arrayptr0 x v);
+  let _ = gen_elim () in
+  let _ = STC.ghost_array_split _ i in
+  let vl_array = {
+    array_ptr = STC.array_split_l v.v_array.array_ptr i;
+    array_perm = v.v_array.array_perm;
+//    array_base_len = v.v_array.array_base_len;
+  }
+  in
+  let vl = {
+    v_array = vl_array;
+    v_contents = Seq.slice v.v_contents 0 (SZ.v i);
+  }
+  in
+  let vr_array = {
+    array_ptr = STC.array_split_r v.v_array.array_ptr i;
+    array_perm = v.v_array.array_perm;
+//    array_base_len = v.v_array.array_base_len;
+  }
+  in
+  let vr = {
+    v_array = vr_array;
+    v_contents = Seq.slice v.v_contents (SZ.v i) (Seq.length v.v_contents);
+  }
+  in
+  let res = Ghost.hide (STC.array_ptr_of vr_array.array_ptr) in
+  STC.array_ref_shift_zero x;
+  let s = vpattern_replace (STC.array_pts_to (STC.array_split_l _ _)) in
+  rewrite (STC.array_pts_to (STC.array_split_l _ _) _) (arrayptr1 vl s);
+  rewrite (arrayptr0 x vl) (arrayptr x vl);
+  let s = vpattern_replace (STC.array_pts_to _) in
+  rewrite (STC.array_pts_to _ _) (arrayptr1 vr s);
+  rewrite (arrayptr0 res vr) (arrayptr res vr);
+  assert (gsplit_post v x i res vl vr);
+  noop ();
+  res
+
+inline_for_extraction [@@noextract_to "krml"]
+let stc_array_ref_split
+  (#t: Type)
+  (#td: STC.typedef t)
+  (#s: Ghost.erased (Seq.seq t))
+  (al: STC.array_ref td)
+  (len: STC.array_len_t al)
+  (aa aal aar: Ghost.erased (STC.array td))
+  (i: SZ.t)
+: ST (_: STC.array_ref td { SZ.v i <= SZ.v len /\ Seq.length s == SZ.v len})
+    (STC.array_pts_to aa s)
+    (fun _ -> STC.array_pts_to aal (Seq.slice s 0 (SZ.v i)) `star`
+      STC.array_pts_to aar (Seq.slice s (SZ.v i) (Seq.length s)))
+    (SZ.v i <= SZ.v len /\
+      Ghost.reveal aa == (| al, len |) /\
+      Ghost.reveal aal == STC.array_split_l aa i /\
+      Ghost.reveal aar == STC.array_split_r aa i
+    )
+    (fun ar ->
+      Ghost.reveal aa == (| al, len |) /\
+      ar == STC.array_ptr_of (STC.array_split_r aa i)
+    )
+= rewrite (STC.array_pts_to aa s) (STC.array_pts_to (| al, len |) s);
+  let res = STC.array_ref_split al len i in
+  vpattern_rewrite (fun a -> STC.array_pts_to a _ `star` STC.array_pts_to (STC.array_split_r _ _) _) aal;
+  vpattern_rewrite (fun a -> STC.array_pts_to aal _ `star` STC.array_pts_to a _) aar;
+  return res
+
+let split' #elt #vl #vr x i x' =
+  rewrite (arrayptr x' vr) (arrayptr0 x' vr);
+  let _ = gen_elim () in
+  rewrite (arrayptr0 x' vr) (arrayptr x' vr);
+  let vm = join x x' in
+  rewrite (arrayptr x vm) (arrayptr0 x vm);
+  let _ = gen_elim () in
+  let res : t elt = stc_array_ref_split x (len vm.v_array) _ vl.v_array.array_ptr vr.v_array.array_ptr i in
+  noop ();
+  rewrite (arrayptr0 x vl) (arrayptr x vl);
+  noop ();
+  rewrite (arrayptr0 res vr) (arrayptr res vr);
+  return res
+
+let index #t #v r i =
+  rewrite (arrayptr r v) (arrayptr0 r v);
+  let _ = gen_elim () in
+  [@@inline_let]
+  let a : STC.array (STC.scalar t) = (| r, Ghost.hide (len v.v_array) |) in
+  let s = vpattern_replace (STC.array_pts_to _) in
+  vpattern_rewrite (fun a -> STC.array_pts_to a _) a;
+  let p = STC.array_cell a i in
+  let res = STC.read p in
+  let _ = STC.unarray_cell a i p in
+  drop (STC.has_array_cell _ _ _);
+  rewrite (STC.array_pts_to _ _) (arrayptr1 v s);
+  rewrite (arrayptr0 r v) (arrayptr r v);
+  return res
+
+let upd #elt #v r i x =
+  rewrite (arrayptr r v) (arrayptr0 r v);
+  let _ = gen_elim () in
+  [@@inline_let]
+  let a : STC.array (STC.scalar elt) = (| r, Ghost.hide (len v.v_array) |) in
+  vpattern_rewrite (fun a -> STC.array_pts_to a _) a;
+  let p = STC.array_cell a i in
+  STC.write p x;
+  let _ = STC.unarray_cell a i p in
+  drop (STC.has_array_cell _ _ _);
+  let s' = vpattern_replace (STC.array_pts_to _) in
+  let res = {
+    v_array = v.v_array;
+    v_contents = Seq.upd v.v_contents (SZ.v i) x;
+  }
+  in
+  rewrite (STC.array_pts_to _ _) (arrayptr1 res s');
+  rewrite (arrayptr0 r res) (arrayptr r res);
+  return res
+
+let set_array_perm
+  (#t: Type)
+  (a: array t)
+  (p: perm)
+: Ghost (array t)
+    (requires True)
+    (ensures (fun y -> len y == len a /\ array_perm y == p))
+= {
+  a with array_perm = p
+}
+
+let set_array_perm_idem
+  (#t: Type)
+  (a: array t)
+  (p1 p2: perm)
+: Lemma
+  (set_array_perm (set_array_perm a p1) p2 == set_array_perm a p2)
+= ()
+
+let set_array_perm_eq
+  (#t: Type)
+  (a: array t)
+: Lemma
+  (set_array_perm a (array_perm a) == a)
+= ()
+
+let set_array_perm_adjacent
+  (#t: Type)
+  (a1 a2: array t)
+  (p: perm)
+: Lemma
+  (requires (adjacent a1 a2))
+  (ensures (
+    merge_into (set_array_perm a1 p) (set_array_perm a2 p) (set_array_perm (merge a1 a2) p)
+  ))
+= ()
+
+#set-options "--ide_id_info_off"
+
+let share
+  (#opened: _)
+  (#elt: Type)
+  (#x: v elt)
+  (a: t elt)
+  (p1 p2: perm)
+: STGhost (Ghost.erased (v elt & v elt)) opened
+    (arrayptr a x)
+    (fun res -> arrayptr a (fst res) `star` arrayptr a (snd res))
+    (array_perm (array_of x) == p1 `Steel.FractionalPermission.sum_perm` p2)
+    (fun res ->
+      contents_of' (fst res) == contents_of x /\
+      contents_of' (snd res) == contents_of x /\
+      array_of (fst res) == set_array_perm (array_of x) p1 /\
+      array_of (snd res) == set_array_perm (array_of x) p2
+    )
+=
+  rewrite (arrayptr a x) (arrayptr0 a x);
+  let _ = gen_elim () in
+  vpattern_rewrite (STC.array_pts_to _) _;
+  STC.mk_fraction_seq_split_gen _ (mk_full_scalar_seq x.v_contents) x.v_array.array_perm p1 p2;
+  let res1 = {
+    v_array = set_array_perm x.v_array p1;
+    v_contents = x.v_contents;
+  }
+  in
+  let res2 = {
+    v_array = set_array_perm x.v_array p2;
+    v_contents = x.v_contents;
+  }
+  in
+  let res = Ghost.hide (res1, res2) in
+  let s = vpattern_replace (fun s -> STC.array_pts_to _ s `star` STC.array_pts_to _ (STC.mk_fraction_seq _ _ p2)) in
+  rewrite (STC.array_pts_to _ s) (arrayptr1 (fst res) s);
+  rewrite (arrayptr0 a (fst res)) (arrayptr a (fst res));
+  let s = vpattern_replace (STC.array_pts_to _) in
+  rewrite (STC.array_pts_to _ _) (arrayptr1 (snd res) s);
+  rewrite (arrayptr0 a (snd res)) (arrayptr a (snd res));
+  res
+
+let gather
+  (#opened: _)
+  (#elt: Type)
+  (#x1 #x2: v elt)
+  (a: t elt)
+: STGhost (v elt) opened
+    (arrayptr a x1 `star` arrayptr a x2)
+    (fun res -> arrayptr a res)
+    (array_of x1 == set_array_perm (array_of x2) (array_perm (array_of x1)))
+    (fun res ->
+      contents_of' res == contents_of x1 /\
+      contents_of' res == contents_of x2 /\
+      array_of res == set_array_perm (array_of x1) (array_perm (array_of x1) `Steel.FractionalPermission.sum_perm` array_perm (array_of x2))
+    )
+= rewrite (arrayptr a x1) (arrayptr0 a x1);
+  let _ = gen_elim () in
+  rewrite (STC.array_pts_to _ _) (STC.array_pts_to x1.v_array.array_ptr (STC.mk_fraction_seq (STC.scalar elt) (mk_full_scalar_seq x1.v_contents) x1.v_array.array_perm));
+  rewrite (arrayptr a x2) (arrayptr0 a x2);
+  let _ = gen_elim () in
+  rewrite
+    (STC.array_pts_to x2.v_array.array_ptr _)
+    (STC.array_pts_to x1.v_array.array_ptr (STC.mk_fraction_seq (STC.scalar elt) (mk_full_scalar_seq x2.v_contents) x2.v_array.array_perm));
+  STC.array_fractional_permissions_theorem (mk_full_scalar_seq x1.v_contents) (mk_full_scalar_seq x2.v_contents) x1.v_array.array_perm x2.v_array.array_perm x1.v_array.array_ptr;
+  rewrite
+    (STC.array_pts_to x1.v_array.array_ptr (STC.mk_fraction_seq (STC.scalar elt) (mk_full_scalar_seq x2.v_contents) x2.v_array.array_perm))
+    (STC.array_pts_to x1.v_array.array_ptr (STC.mk_fraction_seq (STC.scalar elt) (mk_full_scalar_seq x1.v_contents) x2.v_array.array_perm));
+  STC.mk_fraction_seq_join x1.v_array.array_ptr (mk_full_scalar_seq x1.v_contents) x1.v_array.array_perm x2.v_array.array_perm;
+  let s = vpattern_replace (STC.array_pts_to _) in
+  let res = {
+    v_array = set_array_perm x1.v_array (x1.v_array.array_perm `Steel.FractionalPermission.sum_perm` x2.v_array.array_perm);
+    v_contents = x1.v_contents;
+  }
+  in
+  let prf
+    (i: nat)
+  : Lemma
+    (requires (i < length x1.v_array))
+    (ensures (
+      i < length x1.v_array /\
+      Seq.index x1.v_contents i == Seq.index x2.v_contents i
+    ))
+  = STC.mk_scalar_inj (Seq.index x1.v_contents i) (Seq.index x2.v_contents i) full_perm full_perm
+  in
+  Classical.forall_intro (Classical.move_requires prf);
+  assert (x2.v_contents `Seq.equal` x1.v_contents);
+  rewrite (STC.array_pts_to _ _) (arrayptr1 res s);
+  rewrite (arrayptr0 a res) (arrayptr a res);
+  res
